src/program_proof/simple/proofs.v
@@ -1,2 +1,2 @@
 From Perennial.program_proof.simple Require Export
-  common read write getattr setattr.
+  common read write getattr setattr recovery.
