src/program_proof/simple/recovery.v
@@ -1,0 +1,224 @@
+From RecordUpdate Require Import RecordSet.
+Import RecordSetNotations.
+
+From Perennial.algebra Require Import deletable_heap liftable auth_map.
+From Perennial.Helpers Require Import Transitions.
+From Perennial.program_proof Require Import proof_prelude.
+
+From Goose.github_com.mit_pdos.goose_nfsd Require Import simple.
+From Perennial.program_proof Require Import txn.txn_proof marshal_proof addr_proof crash_lockmap_proof addr.addr_proof buf.buf_proof.
+From Perennial.program_proof Require Import buftxn.sep_buftxn_proof buftxn.sep_buftxn_recovery_proof.
+From Perennial.program_proof Require Import proof_prelude.
+From Perennial.program_proof Require Import disk_lib.
+From Perennial.Helpers Require Import NamedProps Map List range_set.
+From Perennial.algebra Require Import log_heap.
+From Perennial.program_logic Require Import spec_assert.
+From Perennial.goose_lang.lib Require Import slice.typed_slice into_val.
+From Perennial.program_proof.simple Require Import spec invariant common.
+From Perennial.goose_lang Require Import crash_modality.
+
+Section stable.
+Context `{!heapG Σ}.
+Context `{!gen_heapPreG u64 bool Σ}.
+Context `{!simpleG Σ}.
+
+Global Instance is_inode_stable_set_stable γsrc γ':
+    IntoCrash ([∗ set] a ∈ covered_inodes, is_inode_stable γsrc γ' a)
+              (λ _, ([∗ set] a ∈ covered_inodes, is_inode_stable γsrc γ' a))%I.
+Proof. rewrite /IntoCrash. iApply post_crash_nodep. Qed.
+
+Global Instance is_txn_durable_stable γ dinit logm:
+    IntoCrash (is_txn_durable γ dinit logm) (λ _, is_txn_durable γ dinit logm).
+Proof.
+  rewrite /IntoCrash. iNamed 1.
+  iDestruct (post_crash_nodep with "Hlogm") as "Hlogm".
+  iDestruct (post_crash_nodep with "Hasync_ctx") as "Hasync_ctx".
+  iCrash. rewrite /is_txn_durable. iFrame.
+Qed.
+
+End stable.
+
+Section heap.
+Context `{!heapG Σ}.
+Context `{!gen_heapPreG u64 bool Σ}.
+Context `{!simpleG Σ}.
+Implicit Types (stk:stuckness) (E: coPset).
+
+Context (P1 : SimpleNFS.State → iProp Σ).
+Context (P2 : SimpleNFS.State → iProp Σ).
+
+Lemma is_source_later_upd P P' γsrc:
+  (∀ σ, ▷ P σ -∗ |C={⊤ ∖ ↑N}_10=> ▷ P σ ∗ ▷ P' σ) -∗
+   ▷ is_source P γsrc -∗
+   |C={⊤}_10=> ▷ is_source P' γsrc.
+Proof.
+  iIntros "Hwand H". iDestruct "H" as (?) "(>?&>%&>#?&?)".
+  iSpecialize ("Hwand" with "[$]").
+  iMod (cfupd_weaken_all with "Hwand") as "(HP1&HP2)"; auto.
+  iModIntro.
+  iNext. iExists _. iFrame "# ∗ %".
+Qed.
+
+Lemma crash_upd_src γsrc γ' src:
+  dom (gset u64) src = covered_inodes →
+  ("Hlmcrash" ∷ ([∗ set] y ∈ covered_inodes, is_inode_stable γsrc γ' y) ∗
+  "Hsrcheap" ∷ map_ctx γsrc 1 src) ==∗
+  ∃ γsrc',
+  map_ctx γsrc 1 src ∗
+  map_ctx γsrc' 1 src ∗
+  [∗ set] y ∈ covered_inodes, is_inode_stable γsrc' γ' y.
+Proof.
+  iIntros (Hdom) "H". iNamed "H".
+  iMod (map_init ∅) as (γsrc') "H".
+  iMod (map_alloc_many src with "H") as "(Hctx&Hmapsto)".
+  { intros. rewrite lookup_empty //=. }
+  rewrite right_id_L.
+  iModIntro. iExists γsrc'.
+  rewrite -Hdom -?big_sepM_dom.
+  iFrame "Hctx".
+  iCombine "Hmapsto Hlmcrash" as "H".
+  rewrite -big_sepM_sep.
+  iApply (big_sepM_mono_with_inv with "Hsrcheap H").
+  iIntros (k v Hlookup) "(Hctx&src&Hstable)".
+  iNamed "Hstable".
+  iDestruct (map_valid with "[$] [$]") as %Heq.
+  subst. iFrame. iExists _. iFrame. rewrite /named. iExactEq "src". f_equal. congruence.
+Qed.
+
+Definition fs_cfupd_cancel dinit P :=
+  (<disc> (|C={⊤}_10=>
+    ∃ γ γsrc logm',
+    is_txn_durable γ dinit logm' ∗
+    ▷ is_source P γsrc ∗
+    [∗ set] a ∈ covered_inodes, is_inode_stable γsrc γ a))%I.
+
+Theorem wpc_Recover γ γsrc (d : loc) dinit logm :
+  {{{
+    <disc> (∀ σ, ▷ P1 σ -∗ |C={⊤ ∖ ↑N}_10=> ▷ P1 σ ∗ ▷ P2 σ) ∗
+    is_txn_durable γ dinit logm ∗
+    ▷ is_source P1 γsrc ∗
+    [∗ set] a ∈ covered_inodes, is_inode_stable γsrc γ a
+  }}}
+    Recover #d @ 10; ⊤
+  {{{ γsimp nfs, RET #nfs;
+      is_fs P1 γsimp nfs dinit ∗ fs_cfupd_cancel dinit P2 }}}
+  {{{
+    ∃ γ' γsrc' logm',
+    is_txn_durable γ' dinit logm' ∗
+    ▷ is_source P2 γsrc' ∗
+    [∗ set] a ∈ covered_inodes, is_inode_stable γsrc' γ' a
+  }}}.
+Proof using All.
+  iIntros (Φ Φc) "(Hshift & Htxndurable & Hsrc & Hstable) HΦ".
+  iMod (fupd_later_to_disc with "Hsrc") as "Hsrc".
+  rewrite /Recover.
+  iApply wpc_cfupd.
+  wpc_pures.
+  { iDestruct "HΦ" as "[HΦc _]". iModIntro.
+    iMod (is_source_later_upd P1 P2 with "Hshift Hsrc") as "Hsrc".
+    iModIntro. iApply "HΦc".
+    iExists _, _, _. iFrame. }
+
+  wpc_apply (wpc_MkTxn Nbuftxn with "Htxndurable").
+  { solve_ndisj. }
+  { solve_ndisj. }
+
+  iSplit.
+  { iDestruct "HΦ" as "[HΦc _]". iModIntro. iIntros "H".
+    iDestruct "H" as (γ' logm') "(%Hkinds & Htxndurable)".
+    iDestruct "Htxndurable" as "(Hdurable&[%Heq|#Hexch])".
+    { subst.
+      iMod (is_source_later_upd P1 P2 with "[$] Hsrc") as "Hsrc".
+      iModIntro. iApply "HΦc". iExists _, _, _.
+      iFrame. }
+    iMod (big_sepS_impl_cfupd with "Hstable []") as "Hcrash".
+    { iModIntro. iIntros (x Hx) "H".
+      iApply (is_inode_stable_crash with "[$] H").
+    }
+    iMod (is_source_later_upd P1 P2 with "[$] Hsrc") as "Hsrc".
+    iModIntro.
+    iApply "HΦc".
+    iExists _, _, _. iFrame.
+  }
+
+  iModIntro.
+  iIntros (γ' l) "(#Histxn & #Htxnsys & Hcfupdcancel & #Htxncrash)".
+
+  wpc_pures.
+  { iDestruct "HΦ" as "[HΦc _]". iModIntro.
+    iMod (big_sepS_impl_cfupd with "Hstable []") as "Hcrash".
+    { iModIntro. iIntros (x Hx) "H".
+      iMod (is_inode_stable_crash with "Htxncrash H") as "H".
+      iModIntro. iExact "H". }
+    iMod "Hcfupdcancel" as ">Hcfupdcancel".
+    iMod (is_source_later_upd P1 P2 with "[$] Hsrc") as "Hsrc".
+    iModIntro.
+    iApply "HΦc".
+    iDestruct "Hcfupdcancel" as (?) "H".
+    iExists _, _, _. iFrame.
+  }
+
+  wpc_apply (wpc_MkLockMap _ covered_inodes (is_inode_stable γsrc γ) (is_inode_stable γsrc γ') with "[Hstable]").
+  { iApply (big_sepS_impl with "Hstable").
+    iModIntro.
+    iIntros (a Ha) "H". iFrame.
+    iModIntro. iIntros ">Hstable".
+    iMod (is_inode_stable_crash with "Htxncrash Hstable") as "Hstable".
+    iModIntro. done. }
+
+  iSplit.
+  { iDestruct "HΦ" as "[HΦc _]". iModIntro. iIntros "H".
+    rewrite -big_sepS_later.
+    iDestruct "H" as ">H".
+    iMod "Hcfupdcancel" as ">Hcfupdcancel".
+    iDestruct "Hcfupdcancel" as (?) "Hcfupdcancel".
+    iMod (is_source_later_upd P1 P2 with "[$] Hsrc") as "Hsrc".
+    iModIntro.
+    iApply "HΦc".
+    iExists _, _, _. iFrame.
+  }
+
+  iModIntro.
+  iIntros (lm ghs) "[#Hlm Hlmcrash]".
+
+  iMod (own_disc_fupd_elim with "Hsrc") as "Hsrc".
+  iMod (inv_alloc N with "Hsrc") as "#Hsrc".
+
+  iApply wp_wpc_frame'.
+  iSplitL "Hlmcrash Hcfupdcancel HΦ Hsrc Hshift".
+  {
+    iAssert (fs_cfupd_cancel dinit P2)%I with "[-HΦ]" as "Hcancel".
+    { iModIntro.
+      rewrite -big_sepS_later.
+      iMod "Hlmcrash" as ">Hlmcrash". iMod "Hcfupdcancel" as ">Hcfupdcancel".
+      iIntros "#HC".
+      iInv "Hsrc" as "Hopen" "Hclose".
+      iDestruct "Hopen" as (?) "(>Hsrcheap&>%Hdom&>#Hnooverflow&HP)".
+      iMod (crash_upd_src with "[$]") as (γsrc') "(Hsrcheap&Hsrcheap'&Hlmcrash)".
+      { eauto. }
+      iMod ("Hshift" with "HP HC") as "(HP1&HP2)".
+      iMod ("Hclose" with "[HP1 Hsrcheap]") as "_".
+      { iNext. iExists _. iFrame "# ∗ %". }
+      iDestruct "Hcfupdcancel" as (?) "?".
+      iExists γ', γsrc', _. iFrame.
+      iModIntro. iNext. iExists _. iFrame "# ∗ %".
+    }
+    iSplit.
+    { iDestruct "HΦ" as "[HΦc _]". iModIntro. iMod ("Hcancel"). iModIntro. by iApply "HΦc". }
+    { iNamedAccu. }
+  }
+
+  wp_apply wp_allocStruct; first by eauto.
+  iIntros (nfs) "Hnfs".
+
+  iDestruct (struct_fields_split with "Hnfs") as "Hnfs". iNamed "Hnfs".
+  iMod (readonly_alloc_1 with "t") as "#Ht".
+  iMod (readonly_alloc_1 with "l") as "#Hl".
+
+  iAssert (is_fs P1 (Build_simple_names γ γ' γsrc ghs) nfs dinit) with "[]" as "Hfs".
+  { iExists _, _. iFrame "Ht Hl Histxn Htxnsys Htxncrash Hlm Hsrc". }
+  wp_pures. iNamed 1.
+  iRight in "HΦ". iApply "HΦ". iFrame "# ∗".
+Qed.
+
+End heap.
